\begin{eqnarray*}
x_{k} &=& f (x_{k-1}, u_{k-1}) + w_{k-1} \\
y_{k} &=& h (x_{k}) + v_{k}
\end{eqnarray*}

\begin{eqnarray*}
\hat{x}_{k|k-1} &=& f (\hat{x}_{k-1|k-1}, u_{k-1})\\
P_{k|k-1} &=& F_{k-1}\ P_{k-1|k-1} F_{k-1}^T + Q
\end{eqnarray*}

\begin{eqnarray*}
z_{k} &=& y_{k} - H\ \hat{x}_{k|k-1} \\
S_{k} &=& H_{k}\ P_{k|k-1} H_{k}^T + R \\
K_{k} &=& P_{k|k-1} H_{k}^T S_{k}^{-1} \\
\hat{x}_{k|k} &=& \hat{x}_{k|k-1}  + K_{k}\ z_{k} \\
P_{k|k} &=& (I - K_{k} H_{k}) P_{k|k-1}
\end{eqnarray*}

$$
F_{k-1} = \frac{\partial f}{\partial x} (\hat{x}_{k-1|k-1}, u_{k-1})
$$
$$
H_{k} = \frac{\partial h}{\partial x} (\hat{x}_{k-1|k-1})
$$
